Do bool_step_prop4 exercise in Smallstep

Smallstep.v
@@ -798,6 +798,8 @@ Inductive step : tm -> tm -> Prop :=
   | ST_If : forall t1 t1' t2 t3,
       t1 ==> t1' ->
       tif t1 t2 t3 ==> tif t1' t2 t3
+  | ST_IfEq : forall t1 t2,
+      tif t1 t2 t2 ==> t2
 (* FILL IN HERE *)
 
   where " t '==>' t' " := (step t t').
@@ -814,7 +816,8 @@ Definition bool_step_prop4 :=
 Example bool_step_prop4_holds :
   bool_step_prop4.
 Proof.
-  (* FILL IN HERE *) Admitted.
+  unfold bool_step_prop4. apply ST_IfEq.
+Qed.
 (** [] *)
 
 (** **** Exercise: 3 stars, optional (properties_of_altered_step) *)
